contrib/subtac/test/take.v
@@ -1,33 +1,38 @@
+(* -*- coq-prog-args: ("-emacs-U" "-debug") -*- *)
 Require Import JMeq.
 Require Import List.
 Require Import Coq.subtac.Utils.
+
+Set Implicit Arguments.
 
 Program Fixpoint take (A : Set) (l : list A) (n : nat | n <= length l) { struct l } : { l' : list A | length l' = n } :=
   match n with
   | 0 => nil
   | S p => 
     match l with
-    | cons hd tl => let rest := take A tl p in cons hd rest
-    | nil => _
+    | cons hd tl => let rest := take tl p in cons hd rest
+    | nil => !
     end
   end.
 
 Require Import Omega.
 
-Obligations.
-
-Solve Obligations using (subtac_simpl ; subst ; auto with arith).
-
-Obligations.
-
-Obligation 3.
-  destruct_call take ; subtac_simpl ; subst ; auto.
-Defined.
-
-Obligation 4.
-  subst l x.
+Next Obligation.
+  intros.
   simpl in l0.
-  absurd (S p <= 0) ; omega.
+  apply le_S_n ; exact l0.
 Defined.
 
-Extraction take.
+Next Obligation.
+  intros.
+  destruct_call take ; subtac_simpl.
+Defined.
+
+Next Obligation.
+  intros.
+  inversion l0.
+Defined.
+
+
+
+
